Towards.v
@@ -3,7 +3,7 @@ Require Import Strings.String.
 Require Import Background.
 
 
-(* `MonadState` generalizes `lens` *)
+(* `MonadState_state` is `identityLn` *)
 
 Definition MonadState_state_2_lens A : lens A A :=
   mkLens (fun a => evalState get a) (fun a a' => execState (put a') a).
@@ -11,6 +11,9 @@ Definition MonadState_state_2_lens A : lens A A :=
 Lemma MonadState_state_is_identity_lens : forall A,
     MonadState_state_2_lens A = identityLn A.
 Proof. auto. Qed.
+
+
+(* Broadly, `MonadState` generalizes `lens` *)
 
 Definition ms_2_lens {S A} (ms : MonadState A (state S)) : lens S A :=
 {| view s     := evalState get s
@@ -22,24 +25,18 @@ Instance lens_2_ms {S A} (ln : lens S A) : MonadState A (state S) :=
 ; put a := mkState (fun s => (tt, update ln s a))
 }.
 
-Ltac i_unfold_behavedness :=
-  unfold very_well_behaved; unfold well_behaved; 
-  unfold view_update; unfold update_view; unfold update_update;
-  unfold get; unfold put;
-  unfold ms_2_lens; unfold lens_2_ms;
-  intros.
-
 Theorem MonadState_state_s_induces_lens : 
     forall {S A : Type} (ms : MonadState A (state S)),
-           @MonadStateLaws A (state S) _ ms -> very_well_behaved (ms_2_lens ms).
+           @MonadStateLaws A (state S) _ ms -> lensLaws (ms_2_lens ms).
 Proof.
-  i_unfold_behavedness.
+  intros.
+  unfold ms_2_lens.
   assert (F : forall s, put (evalState get s) = get >> put (evalState get s)).
   { intros.
     rewrite <- (non_eff_get (put (evalState get s))).
     now rewrite (general_getget (fun _ => put (evalState get s))). }
   destruct H.
-  repeat split; intros; simpl.
+  constructor; intros; simpl.
 
   - (* view_update *)
     rewrite F.
@@ -59,10 +56,10 @@ Qed.
 
 Theorem lens_induces_MonadState_state_s :
     forall {S A : Type} (ln : lens S A),
-           very_well_behaved ln -> @MonadStateLaws A (state S) _ (lens_2_ms ln).
+           lensLaws ln -> @MonadStateLaws A (state S) _ (lens_2_ms ln).
 Proof.
-  i_unfold_behavedness.
-  destruct H as [[view_update update_view] update_update].
+  intros.
+  destruct H.
   split; 
     simpl; 
     intros; 
@@ -72,26 +69,24 @@ Proof.
 Qed.
 
 
-(* Lens Algebra definition *)
+(* Lens Algebra definition, just a record *)
 
 Record lensAlg (p : Type -> Type) (A : Type) `{M : Monad p} : Type :=
-{ (* abstract definitions *)
-  get : p A
+{ get : p A
 ; put : A -> p unit
-
-  (* laws *)
-; get_get : get >>= (fun s1 => get >>= (fun s2 => ret (s1, s2))) =
-            get >>= (fun s => ret (s, s))
-; get_put : get >>= put = ret tt
-; put_get : forall s, put s >> get = put s >> ret s
-; put_put : forall s1 s2, put s1 >> put s2 = put s2
-
-  (* derived methods *)
 ; modify (f : A -> A) : p unit := get >>= (put ∘ f)
 }.
 Arguments get [p A _].
 Arguments put [p A _].
 Arguments modify [p A _].
+
+Record lensAlgLaws {p A} `{Monad p} (ln : lensAlg p A) : Type :=
+{ get_get : get ln >>= (fun s1 => get ln >>= (fun s2 => ret (s1, s2))) =
+            get ln >>= (fun s => ret (s, s))
+; get_put : get ln >>= put ln = ret tt
+; put_get : forall s, put ln s >> get ln = put ln s >> ret s
+; put_put : forall s1 s2, put ln s1 >> put ln s2 = put ln s2
+}.
 
 
 (* Zip example *)
